fairness/lawyer/program_logic.v
@@ -9,6 +9,8 @@ From trillium.fairness.lawyer Require Import obligations_model.
 From trillium.fairness.heap_lang Require Import sswp_logic.
 
 
+Close Scope Z. 
+
 Section ProgramLogic.
   Context `{OfeDiscrete DegO} `{OfeDiscrete LevelO}. 
   
@@ -44,15 +46,164 @@ Section ProgramLogic.
           ⌜ locale_step c (Some τ) c' ⌝
     end.
 
+    Definition HL_OM_trace_interp'_step (extr: execution_trace heap_lang)
+      (omtr: auxiliary_trace OM) (τ: locale heap_lang) (k: nat): iProp Σ :=
+      match extr with
+      | {tr[ _ ]} => False
+      | extr' :tr[oζ]: c' =>
+          let c := trace_last extr' in
+          let δ := trace_last omtr in
+          ∃ δ__k,
+          (* ⌜ k <= LIM_STEPS - n⌝ ∗  *)
+          gen_heap_interp c'.2.(heap) ∗
+          obls_msi OP δ__k (H1 := oGS) ∗
+          ⌜ nsteps (fun p1 p2 => ghost_step OP p1 τ p2) k δ δ__k ⌝ ∗
+          ⌜ threads_own_obls OP c δ ⌝ ∗
+          ⌜ oζ = Some τ ⌝ ∗
+          ⌜ locale_step c (Some τ) c' ⌝
+    end.
+
+    
     Definition MU E ζ (P : iProp Σ) : iProp Σ :=
     ∀ extr atr,
       HL_OM_trace_interp' extr atr ζ ={E}=∗
       ∃ δ2 ℓ, state_interp extr (trace_extend atr ℓ δ2) (irisG := @heapG_irisG _ _ _ hGS) ∗ P.
 
+    Lemma burn_cp_upd δ ph deg:
+      ⊢ obls_msi OP δ (H1 := oGS) -∗ cp OP ph deg (H1 := oGS) ==∗ obls_msi OP (update_cps OP (ps_cps OP δ ∖ {[+ (ph, deg) +]}) δ) (H1 := oGS).
+    Proof.
+      iIntros "MSI CP".
+      rewrite {1}/obls_msi. iDestruct "MSI" as "(CPS&?&?&?&?&?)".
+      destruct δ. simpl. iFrame. simpl.
+      rewrite /cp.
+      From iris.algebra Require Import gmultiset.
+      iCombine "CPS CP" as "?". iApply (own_update with "[$]").
+      apply auth_update_dealloc.
+      eapply local_update_proper; [..| eapply gmultiset_local_update_dealloc].
+      1, 3: reflexivity.
+      f_equiv. by rewrite gmultiset_difference_diag.
+    Qed.
+
+    (* ⌜ ps_phases OP δ !! τ = Some π__max /\ phase_le ph π__max /\ *)
+    Lemma cp_msi_dom δ ph deg:
+      ⊢ obls_msi OP δ (H1 := oGS) -∗ cp OP ph deg (H1 := oGS) -∗
+        ⌜ (ph, deg) ∈ ps_cps OP δ ⌝.
+    Proof.
+      rewrite /obls_msi. iIntros "(CPS&_) CP". 
+      iCombine "CPS CP" as "CPS". 
+      iDestruct (own_valid with "[$]") as %V. iPureIntro.
+      apply auth_both_valid_discrete, proj1 in V.
+      apply gmultiset_singleton_subseteq_l.
+      by apply gmultiset_included.
+    Qed. 
+
+    (* TODO: clarify how to derive this fact *)
+    Lemma WIP_th_own_ex_phase c τ c' δ
+      (STEP: locale_step c (Some τ) c')
+      (OBLS: threads_own_obls OP c δ):
+      exists π, ps_phases OP δ !! τ = Some π.
+    Proof. Admitted.
+
+    (* TODO: ghost steps should preserve it *)
+    Lemma WIP_th_own_gsteps_ex_phase c τ c' δ δ' n
+      (STEP: locale_step c (Some τ) c')
+      (OBLS: threads_own_obls OP c δ)
+      (GSTEPS: relations.nsteps (fun p1 p2 => ghost_step OP p1 τ p2) n δ δ'):
+      exists π, ps_phases OP δ' !! τ = Some π.
+    Proof. Admitted.
+
+    Lemma WIP_all_phases_le π1 π2:
+      phase_le π1 π2.
+    Proof. done. Qed. 
+
+    Lemma finish_obls_steps extr omtr τ n ph deg
+      (BOUND: n <= LIM_STEPS)
+      :
+      ⊢ HL_OM_trace_interp'_step extr omtr τ n -∗ (cp OP ph deg (H1 := oGS)) ==∗
+        ∃ δ', state_interp extr (trace_extend omtr τ δ') (irisG := @heapG_irisG _ _ _ hGS).
+    Proof.
+      iIntros "TI'' cp". rewrite /HL_OM_trace_interp'_step.
+      destruct extr; [done| ].
+      iDestruct "TI''" as (δ__k) "(HEAP&MSI&%TRANSS&%OBLS&->&%STEP)".
+      iDestruct (cp_msi_dom with "[$] [$]") as %CP. 
+      iMod (burn_cp_upd with "[$] [$]") as "X".
+      iModIntro. iExists _. simpl. iFrame.
+      
+      pose proof (WIP_th_own_gsteps_ex_phase _ _ _ _ _ _ STEP OBLS TRANSS) as [πτ PHτ]. 
+
+      assert (threads_own_obls OP a (update_cps OP (ps_cps OP δ__k ∖ {[+ (ph, deg) +]}) δ__k)) as TH_OWN'.
+      { eapply locale_step_th_obls_pres in OBLS; eauto.
+        remember (trace_last extr) as X.
+        destruct X as [??], a as [??].
+        eapply progress_step_th_obls_pres with (τ := τ); eauto.
+        2: { eapply from_locale_step; eauto.
+             admit. }
+        eexists. split; eauto.
+        eexists. split; eauto.
+        do 2 eexists. econstructor; eauto.
+        apply WIP_all_phases_le. }
+      
+      iPureIntro. split; auto. 
+      
+      red. repeat split; auto.
+      simpl. red. eexists. split; eauto.
+      eexists. split; eauto. do 2 eexists. econstructor; eauto.
+      apply WIP_all_phases_le. 
+      
+    Admitted. 
+
+    (* Definition SMU E ζ n (P : iProp Σ) : iProp Σ := *)
+    (* ∀ extr atr, *)
+    (*   HL_OM_trace_interp'_step extr atr ζ n ={E}=∗ *)
+    (*   ∃ δ2 ℓ, state_interp extr (trace_extend atr ℓ δ2) (irisG := @heapG_irisG _ _ _ hGS) ∗ P. *)
+
+    (* TODO: figure out the correct inequalities *)
+    Definition BMU E ζ b (P : iProp Σ) : iProp Σ :=
+    ∀ extr atr n,
+      (* ⌜ n <= LIM_STEPS - b ⌝ ∗ *)
+      HL_OM_trace_interp'_step extr atr ζ n ={E}=∗
+      ∃ n', HL_OM_trace_interp'_step extr atr ζ n' ∗ 
+            (* ⌜ n <= n' <= LIM_STEPS ⌝ ∗  *)
+            ⌜ n' - n <= b ⌝ ∗
+            P.
+
+    (* TODO: should we ex quantify ph and deg under BMU? *)
+    Lemma BMU_MU E ζ b (P : iProp Σ) ph deg
+      (BOUND: b <= LIM_STEPS)
+      :
+      BMU E ζ b (cp OP ph deg (H1 := oGS) ∗ P) ⊢ MU E ζ P.
+    Proof.
+      rewrite /MU /BMU. iIntros "BMU" (etr otr) "TI'".
+      iSpecialize ("BMU" $! etr otr 0 with "[TI']").
+      { rewrite /HL_OM_trace_interp' /HL_OM_trace_interp'_step.
+        destruct etr; [done| ].
+        iDestruct "TI'" as "(HEAP&MSI&%OBLS&->&%STEP)".
+        iExists _. iFrame. iPureIntro.
+        repeat split; try done.
+        econstructor. }
+      iMod "BMU" as (n') "(TI'' & %BOUND' & CP & P)". iFrame.
+      iMod (finish_obls_steps with "[$] [$]") as (?) "?".
+      { lia. }       
+      iModIntro. eauto.
+    Qed.
+
+    (* Lemma BMU_step_burn E ζ n P ph deg: *)
+    (*    ⊢ BMU E ζ n P -∗ cp OP ph deg (H1 := oGS) -∗ BMU E ζ (S n) P. *)
+    (* Proof.  *)
+
+    Definition sgn (sid: SignalId) (l: Level) (b: bool): iProp Σ.
+    Admitted. 
+
+    Lemma BMU_step_create_signal E ζ P n l:
+       ⊢ (∀ sid, sgn sid l false -∗ BMU E ζ n P) -∗ BMU E ζ (S n) P.
+    Proof.
+      iIntros "CONT". rewrite /BMU.
+    Abort. 
+    
     Lemma sswp_MU_wp_fupd s E E' ζ e Φ
       (NVAL: language.to_val e = None)
       :
-      let sswp_post := λ e', (MU E' ζ ((|={E',E}=> WP e' @ s; ζ; E {{ Φ }})))%I in
+      let sswp_post := λ e', (MU E' ζ (|={E',E}=> WP e' @ s; ζ; E {{ Φ }}))%I in
       (|={E,E'}=> sswp s E' e sswp_post)%I -∗
         WP e @ s; ζ; E {{ Φ }}.
     Proof.
